nola/examples/logic/adequacy.v
@@ -12,13 +12,15 @@ Class nintpGpreS Σ := NintpGpreS {
   nintpGpreS_cinv :: cinvG Σ;
   nintpGpreS_borrow :: borrowGpreS (nPropS (;ᵞ)) Σ;
   nintpGpreS_fborrow :: fborrowGpreS (nPropS (;ᵞ)) Σ;
+  nintpGpreS_proph :: prophGpreS nsynty Σ;
   nintpGpreS_heap :: heapGpreS Σ;
 }.
 
 (** [gFunctors] for [nintpGpreS] *)
 Definition nintpΣ : gFunctors :=
   #[agreeΣ (nPropL (;ᵞ)); ninvΣ (nPropS (;ᵞ)); na_ninvΣ (nPropS (;ᵞ));
-    na_invΣ; cinvΣ; borrowΣ (nPropS (;ᵞ)); fborrowΣ (nPropS (;ᵞ)); heapΣ].
+    na_invΣ; cinvΣ; borrowΣ (nPropS (;ᵞ)); fborrowΣ (nPropS (;ᵞ));
+    prophΣ nsynty; heapΣ].
 #[export] Instance subG_nintpGpreS `{!subG nintpΣ Σ} : nintpGpreS Σ.
 Proof. solve_inG. Qed.
 
@@ -28,28 +30,30 @@ Definition nwsatd `{!nintpGS Σ} W E c : iProp Σ :=
 
 (** Adequacy of [wp] over [inv_wsatd] *)
 Lemma wp_n_adequacy `{!nintpGpreS Σ} {s e σ φ} :
-  (∀ `{!nintpGS Σ}, ⊢ ∃ W E c, inv_heap_inv -∗
+  (∀ `{!nintpGS Σ}, ⊢ ∃ W E c, proph_ctx -∗ inv_heap_inv -∗
     WP[nwsatd W E c] e @ s; ⊤ {{ v, ⌜φ v⌝ }}) →
   adequate s e σ (λ v _, φ v).
 Proof.
   move=> towp. apply (heap_adequacy Σ HasNoLc)=> ?.
   iMod inv_wsat_alloc as (?) "W0". iMod na_inv_wsat_alloc as (?) "W1".
   iMod borrow_wsat_alloc as (?) "W2". iMod fborrow_wsat_alloc as (?) "W3".
-  iModIntro. iDestruct (towp (NintpGS _ _ _ _ _ _ _ _)) as (W E c) "big".
-  iExists (nwsatd W E c). iFrame "big". iSplitL "W0"; [done|].
-  iSplitL "W1"; [done|]. by iSplitL "W2".
+  iMod proph_init as (?) "PROPH"; [done|]. iModIntro.
+  iDestruct (towp (NintpGS _ _ _ _ _ _ _ _ _)) as (W E c) "big".
+  iExists (nwsatd W E c). iDestruct ("big" with "PROPH") as "$".
+  iSplitL "W0"; [done|]. iSplitL "W1"; [done|]. by iSplitL "W2".
 Qed.
 
 (** Adequacy of [twp] over [inv_wsatd] *)
 Lemma twp_n_adequacy `{!nintpGpreS Σ} {s e σ φ} :
-  (∀ `{!nintpGS Σ}, ⊢ ∃ W E c, inv_heap_inv -∗
+  (∀ `{!nintpGS Σ}, ⊢ ∃ W E c, proph_ctx -∗ inv_heap_inv -∗
     WP[nwsatd W E c] e @ s; ⊤ [{ v, ⌜φ v⌝ }]) →
   sn erased_step ([e], σ).
 Proof.
   move=> totwp. apply (heap_total Σ s _ _ φ)=> ?.
   iMod inv_wsat_alloc as (?) "W0". iMod na_inv_wsat_alloc as (?) "W1".
   iMod borrow_wsat_alloc as (?) "W2". iMod fborrow_wsat_alloc as (?) "W3".
-  iModIntro. iDestruct (totwp (NintpGS _ _ _ _ _ _ _ _)) as (W E c) "big".
-  iExists (nwsatd W E c). iFrame "big". iSplitL "W0"; [done|].
-  iSplitL "W1"; [done|]. by iSplitL "W2".
+  iMod proph_init as (?) "PROPH"; [done|]. iModIntro.
+  iDestruct (totwp (NintpGS _ _ _ _ _ _ _ _ _)) as (W E c) "big".
+  iExists (nwsatd W E c). iDestruct ("big" with "PROPH") as "$".
+  iSplitL "W0"; [done|]. iSplitL "W1"; [done|]. by iSplitL "W2".
 Qed.
