nola/examples/logic/synty.v
@@ -1,0 +1,88 @@
+(** * Syntactic type *)
+
+From nola.iris Require Export prophecy.
+
+(** Syntactic type *)
+Inductive nsynty := Empty_setₛ | natₛ | Zₛ | boolₛ | unitₛ | Propₛ
+| optionₛ (X : nsynty) | listₛ (X : nsynty) | prodₛ (X Y : nsynty)
+| sumₛ (X Y : nsynty) | funₛ (X Y : nsynty).
+Implicit Type (X Y : nsynty).
+
+Declare Scope nsynty_scope.
+Bind Scope nsynty_scope with nsynty.
+Delimit Scope nsynty_scope with ST.
+Notation "()" := unitₛ : nsynty_scope.
+Infix "*" := prodₛ : nsynty_scope. Infix "+" := sumₛ : nsynty_scope.
+Infix "→" := funₛ : nsynty_scope.
+
+(** Interpret [nsynty] as a type *)
+Fixpoint nsynty_ty (X: nsynty) : Type :=
+  match X with
+  | Empty_setₛ => Empty_set | natₛ => nat | Zₛ => Z | boolₛ => bool
+  | unitₛ => () | Propₛ => Prop | optionₛ X => option (nsynty_ty X)
+  | listₛ X => list (nsynty_ty X) | prodₛ X Y => nsynty_ty X * nsynty_ty Y
+  | sumₛ X Y => nsynty_ty X + nsynty_ty Y
+  | funₛ X Y => nsynty_ty X → nsynty_ty Y
+  end.
+Coercion nsynty_ty: nsynty >-> Sortclass.
+
+(** Decidable equality *)
+#[export] Instance nsynty_eq_dec : EqDecision nsynty.
+Proof. solve_decision. Defined.
+
+(** Decidable inhabitedness *)
+
+Fixpoint nsynty_inhab X : bool :=
+  match X with
+  | Empty_setₛ => false | prodₛ X Y => nsynty_inhab X && nsynty_inhab Y
+  | sumₛ X Y => nsynty_inhab X || nsynty_inhab Y
+  | funₛ X Y => negb (nsynty_inhab X) || nsynty_inhab Y
+  | _ => true
+  end.
+
+Local Lemma of_either_nsynty_inhab {X} :
+  (nsynty_inhab X → X) * (negb (nsynty_inhab X) → X → False).
+Proof.
+  move: X. fix FIX 1. move=> X. split.
+  - case: X=>//=; try by (move=> *; exact inhabitant).
+    + move=> ?? /andb_True[??]. constructor; by apply FIX.
+    + move=> X ?. case eq: (nsynty_inhab X)=>/= H.
+      * apply inl, FIX. by rewrite eq.
+      * by apply inr, FIX.
+    + move=> X ?. case eq: (nsynty_inhab X)=>/= ??; [by apply FIX|].
+      exfalso. eapply FIX; [|done]. by rewrite eq.
+  - case: X=>//=.
+    + move=> X ?. rewrite negb_andb.
+      case eq: (nsynty_inhab X)=>/= ?[a?]; [by eapply FIX|].
+      eapply FIX; [|apply a]. by rewrite eq.
+    + move=> ??. by rewrite negb_orb=> /andb_True[??] [a|b];
+      eapply FIX; [|apply a| |apply b].
+    + move=> ??. rewrite negb_orb negb_involutive=> /andb_True[??] f.
+      eapply FIX; [done|]. by apply f, FIX.
+Qed.
+Lemma of_nsynty_inhab {X} : nsynty_inhab X → X.
+Proof. apply of_either_nsynty_inhab. Qed.
+Lemma of_neg_nsynty_inhab {X} : negb (nsynty_inhab X) → X → False.
+Proof. apply of_either_nsynty_inhab. Qed.
+Lemma to_nsynty_inhab {X} (x: X) : nsynty_inhab X.
+Proof.
+  case eq: (nsynty_inhab X); [done|]. exfalso.
+  eapply of_neg_nsynty_inhab; [|done]. by rewrite eq.
+Qed.
+Lemma to_neg_nsynty_inhab {X} (f: X → False) : negb (nsynty_inhab X).
+Proof.
+  case eq: (nsynty_inhab X); [|done]. exfalso. apply f, of_nsynty_inhab.
+  by rewrite eq.
+Qed.
+
+(** [nsynty] is [synty] *)
+Program Canonical nsynty_synty : synty := {|
+  synty_car := nsynty; synty_ty := nsynty_ty; synty_inhab := nsynty_inhab;
+|}.
+Next Obligation. by move=> ? /of_nsynty_inhab. Qed.
+Next Obligation. by move=> ? /to_nsynty_inhab. Qed.
+
+Notation prvarn := (prvar nsynty).
+Notation aprvarn := (aprvar nsynty).
+Notation proph_asnn := (proph_asn nsynty).
+Notation prophn A := (proph nsynty A).
